theories/examples/increment.v
@@ -1,0 +1,35 @@
+From ltl Require Import ltl ltl_fixpoints ltl_now.
+
+Section increment_example.
+  Definition state := nat.
+  Definition label := unit.
+  Inductive steps : state → label → state → Prop :=
+    | my_step i : steps i () (i+1).
+
+  Notation tProp := (tProp state label steps).
+
+  Lemma step : ⊢ ∀ i, ↓s i → ○ ↓s (i+1) : tProp.
+  Proof.
+    iIntros (i) "H".
+    iDestruct (trace_steps_det with "H") as "[Hl Hs]".
+    { intros. by inversion H; inversion H0; simplify_eq. }
+    { econstructor. }
+    done.
+  Qed.
+
+  Lemma eventually_n (n:nat) : ↓s 0 ⊢ ◊ ↓s n : tProp.
+  Proof.
+    iDestruct step as "Hstep".
+    assert (∃ i j, i = 0 ∧ n = i+j) as (i&j&Heq&H1).
+    { eexists 0, n. lia. }
+    rewrite -{2}Heq. clear Heq.
+    iInduction j as [|j IH] forall (i H1).
+    { simplify_eq. rewrite right_id. iIntros "Hs". iModIntro. iApply "Hs". }
+    iIntros "Hs".
+    iDestruct (step with "Hs") as "Hs".
+    iApply ltl_next_eventually. iModIntro.
+    iApply ("IH" with "[] Hs").
+    iPureIntro. lia.
+  Qed.
+
+End increment_example.
