theories/examples/petri_nets.v
@@ -1,4 +1,4 @@
-From ltl Require Import ltl ltl_fixpoints ltl_now ltl_adequacy classical.
+From ltl Require Import ltl ltl_fixpoints ltl_now ltl_adequacy.
 
 Import tProp.
 
