theories/examples/yes_no.v
@@ -1,0 +1,75 @@
+From ltl Require Import ltl ltl_fixpoints ltl_now classical.
+
+Module yes_no_example.
+
+  Definition state : Set := nat * bool.
+  Definition label : Set := bool.
+  Inductive steps : state → label → state → Prop :=
+  | step_succ i b : i > 0 → steps (i,b) b (i-1,negb b)
+  | step_fail i b : i > 0 → steps (i,b) (negb b) (i,b).
+
+  Notation tProp := (tProp state label steps).
+
+  Lemma inf_live b :
+    ∞ ⊢@{tProp} □ ◊ is_live b.
+  Proof.
+    iApply inf_live_strong.
+    intros. inversion H; [destruct b'|destruct b0]; destruct b; simplify_eq; eexists _; econstructor; lia.
+  Qed.
+
+  Axiom fair : ∀ (b:bool),
+    ⊢ (□ ◊ is_live b) → ◊ ↓l b : tProp.
+
+  Lemma step_b b i :
+    ↓s (S i,b) ⊢ ↓l b ∧ ○ ↓s (S i - 1,negb b) ∨ ↓l (negb b) ∧ ○ (↓s (S i,b)) : tProp.
+  Proof.
+    iIntros "H".
+    iDestruct (trace_steps with "H") as (l s' Hsteps') "[Hl Hs]";
+      [by eexists _, _; constructor; lia|].
+    inversion Hsteps'; simplify_eq.
+    - iLeft. iFrame.
+    - iRight. iFrame.
+  Qed.
+
+  Lemma step_b_label b i :
+    ↓s (S i,b) ∧ ↓l b ⊢  ○ ↓s (S i - 1, negb b): tProp.
+  Proof.
+    iIntros "[Hs Hl]".
+    iDestruct (trace_steps_label with "[$Hs $Hl]") as (s' Hsteps') "Hs".
+    inversion Hsteps'; simplify_eq.
+    - done.
+    - by destruct b.
+  Qed.
+
+  Theorem eventually_terminates (n:nat) :
+    ↓fs fst n ⊢@{tProp} ◊ ↯.
+  Proof.
+    rewrite (ltl_eventually_intro_now (↓fs fst n)).
+    iInduction n as [|n IHn].
+    { iIntros ">Hs".
+      iDestruct (ltl_now_prod_fst with "Hs") as (b) "Hs".
+      iDestruct (trace_terminates with "Hs") as "Hs".
+      { intros H. inversion H as (?&?&?). inversion H0; lia. }
+      rewrite -ltl_next_eventually. iModIntro. iModIntro. done. }
+    iIntros ">Hs".
+    iDestruct (ltl_now_prod_fst with "Hs") as (b) "Hs".
+    iDestruct ltl_terminates_dec as "[$|#H]".
+    iApply "IHn". iClear "IHn".
+    iDestruct (inf_live b with "H") as "#Hlive".
+    iDestruct (fair with "Hlive") as "-#Hsched".
+    iRevert "Hs".
+    iApply (ltl_eventually_ind_strong with "[] Hsched").
+    iIntros "!> [Hl|[_ IH]] Hs".
+    { iDestruct (step_b_label with "[$Hs $Hl]") as "H'".
+      iEval (rewrite -ltl_next_eventually). iModIntro. iModIntro.
+      iApply ltl_now_prod_fst. iExists _.
+      replace (S n - 1) with n by lia. done. }
+    iDestruct (step_b with "Hs") as "[[Hl Hs]|[Hl Hs]]".
+    - iEval (rewrite -ltl_next_eventually). iModIntro. iModIntro.
+      iApply ltl_now_prod_fst. iExists _.
+      replace (S n - 1) with n by lia. done.
+    - iEval (rewrite -ltl_next_eventually). iModIntro.
+      by iApply "IH".
+  Qed.
+
+End yes_no_example.
